src/proofs/ElimLet.v
@@ -9,5 +9,108 @@ really the primary difference between the two layers) so it does encompass the m
 difficulties.
 *)
 Require Import TaskDefs.
+Require Import TermTraverse.
 
 (*First, define the stateful transformation*)
+
+Import MonadNotations.
+
+Local Open Scope errst_scope.
+
+(*Simple: eliminate all*)
+Check term_map.
+Definition elim_let_rewrite (t: term_c) : errState (CoqBigInt.t * hashcons_full) term_c :=
+  term_map hashcons_full
+  (*let is only interesting one*)
+  (fun t1 t2 t3 v r1 r2 =>
+    t_subst_single1 v r1 r2)
+  (tmap_if_default _)
+  (tmap_app_default _)
+  (tmap_match_default _)
+  (tmap_eps_default _)
+  (tmap_quant_default _)
+  (tmap_binop_default _)
+  (tmap_not_default _)
+  t.
+
+(*And the transformation*)
+
+
+(*Change decl in task_hd*)
+
+Definition change_tdecl_node (t: tdecl_c) (new: tdecl_node) : tdecl_c :=
+  mk_tdecl_c new (td_tag_of t).
+
+Definition change_tdecl_c (t: task_hd) (new: tdecl_c) : task_hd :=
+  mk_task_head new (task_prev t) (task_known t) (task_clone t) (task_meta t) (task_tag t).
+
+Definition change_decl_node (d: decl) (new: decl_node) : decl :=
+  build_decl new (d_news d) (d_tag d).
+
+(*NOTE: assuming goal is at the end (just like with eval)*)
+Definition rewrite_goal {St} (f: prsymbol -> term_c -> errState St term_c)
+  (t: task_hd) : errState St task_hd :=
+  match (td_node_of (task_decl t)) with
+  | Decl d =>
+    match d_node d with
+      | Dprop x =>
+        let '(k, pr, f1) := of_tup3 x in
+        match k with
+        | Pgoal => 
+          f2 <- f pr f1 ;;
+          errst_ret (change_tdecl_c t (change_tdecl_node (task_decl t) (Decl (change_decl_node d (Dprop (k, pr, f2))))))
+        | _ => (*dont do anything*) errst_ret t
+        end
+      | _ => errst_ret t
+      end
+  | _ => errst_ret t
+  end.
+
+Definition elim_let_aux (t: task_hd) : errState (CoqBigInt.t * hashcons_full) task_hd :=
+  rewrite_goal (fun _ => elim_let_rewrite) t.
+
+Require Import TransDefs.
+
+Definition lift_trans (f: task_hd -> errState (CoqBigInt.t * hashcons_full) task_hd) :
+  trans_errst task :=
+  fun t => 
+    match t with
+    | None => errst_ret None
+    | Some t => x <- f t;; errst_ret (Some x)
+    end.
+
+Definition elim_let : trans_errst task := lift_trans elim_let_aux.
+Set Bullet Behavior "Strict Subproofs".
+(*Soundness*)
+Require Import Relations ErrStateHoare StateInvar Soundness.
+Require Import eliminate_let.
+Check trans_errst.
+
+(*The main part: prove related*)
+Theorem elim_let_related (tsk1 : task) (tsk2 : Task.task):
+errst_spec
+  (fun s : full_st => st_wf tsk1 s /\ task_related tsk1 tsk2)
+  (elim_let tsk1)
+  (fun (_ : full_st) (r : task) (_ : full_st) =>
+   task_related r (single_goal (elim_let_f true true) tsk2)).
+Proof.
+  (*need to do induction on formula*)
+  (*Next steps:
+    1. prove we can move [task_related] out of condition (or maybe just change decomp?
+    2. unfold tasks, get elim_let and elim_let_f just on goal,
+      then need to get formulas, do induction on formulas
+      will need to reason about eval, related, and results via induction
+      do not want to unfold errst_spec if possible so we can prove intermediate results
+  unfold task_related at 1.
+  unfold errst_spec.
+
+
+
+
+Theorem elim_let_sound: trans_errst_sound elim_let.
+Proof.
+  apply prove_trans_errst_decompose with (tr1:=single_goal (elim_let_f true true)).
+  - (*already proved soundness*) apply elim_let_sound. 
+  - (*Now prove related*)
+
+
